fix havoc (need to instantiate type variables in specified type using type environment)

BoogieLang/Semantics.thy
@@ -303,7 +303,7 @@ inductive red_cmd :: "'a absval_ty_fun \<Rightarrow> method_context \<Rightarrow
   | RedAssign: "\<lbrakk>A,\<Lambda>,\<Gamma>,\<Omega> \<turnstile> \<langle>e, n_s\<rangle> \<Down> v \<rbrakk> \<Longrightarrow>
                A,M,\<Lambda>,\<Gamma>,\<Omega> \<turnstile> \<langle>Assign x e, Normal n_s\<rangle> \<rightarrow>  Normal (update_var \<Lambda> n_s x v)"  
 (* restrict x < length \<Lambda> ? *)
-  | RedHavoc: "\<lbrakk> lookup_var_ty \<Lambda> x = Some ty; type_of_val A v = ty \<rbrakk> \<Longrightarrow>
+  | RedHavoc: "\<lbrakk> lookup_var_ty \<Lambda> x = Some ty; type_of_val A v = instantiate \<Omega> ty \<rbrakk> \<Longrightarrow>
                A,M,\<Lambda>,\<Gamma>,\<Omega> \<turnstile> \<langle>Havoc x, Normal n_s\<rangle> \<rightarrow> Normal (update_var \<Lambda> n_s x v)"  
   | RedMethodCallOk: "\<lbrakk> map_of M m = Some msig; 
       A,\<Lambda>,\<Gamma>,\<Omega> \<turnstile> \<langle>args, n_s\<rangle> [\<Down>] v_args;
@@ -324,6 +324,8 @@ inductive red_cmd :: "'a absval_ty_fun \<Rightarrow> method_context \<Rightarrow
 inductive_cases RedAssertOk_case: "A,M,\<Lambda>,\<Gamma>,\<Omega> \<turnstile> \<langle>Assert e, Normal n_s\<rangle> \<rightarrow> Normal n_s"
 inductive_cases RedAssumeOk_case: "A,M,\<Lambda>,\<Gamma>,\<Omega> \<turnstile> \<langle>Assume e, Normal n_s\<rangle> \<rightarrow> Normal n_s"
 inductive_cases RedAssign_case: "A,M,\<Lambda>,\<Gamma>,\<Omega> \<turnstile> \<langle>Assign x e, Normal n_s\<rangle> \<rightarrow> Normal (update_var \<Lambda> n_s x v)"
+inductive_cases RedHavoc_case: "A,M,\<Lambda>,\<Gamma>,\<Omega> \<turnstile> \<langle>Havoc x, Normal n_s\<rangle> \<rightarrow> Normal (update_var \<Lambda> n_s x v)"
+
 
 inductive red_cmd_list :: "'a absval_ty_fun \<Rightarrow> method_context \<Rightarrow> var_context \<Rightarrow> 'a fun_context \<Rightarrow> rtype_env \<Rightarrow> cmd list \<Rightarrow> 'a state \<Rightarrow> 'a state \<Rightarrow> bool"
   ("_,_,_,_,_ \<turnstile> ((\<langle>_,_\<rangle>) [\<rightarrow>]/ _)" [51,0,0,0] 81)
